coq/Slope_base.v
@@ -1,8 +1,7 @@
 (* Slope_base.v *)
 
-From Stdlib Require Import Utf8.
-Require Import QGArith.
-Open Scope QG.
+From Stdlib Require Import Utf8 ZArith.
 
-Definition slope_expr pt₁ pt₂ :=
-  (snd pt₂ - snd pt₁) / (QG_of_nat (fst pt₂) - QG_of_nat (fst pt₁)).
+Definition slope_expr pt₁ pt₂ den :=
+  ((snd pt₂ - snd pt₁)%Z,
+   (den * Pos.of_nat (fst pt₂ - fst pt₁))%positive).
